src/Eval.v
@@ -1,22 +1,101 @@
-Require Import Coq.Strings.String.
+(*Require Import Ast.*)
+
+Require Import Coq.Init.Datatypes.
 Require Import Coq.Lists.List.
-Require Import Coq.Bool.Bool.
+Require Import Coq.Classes.EquivDec.
+Require Import Coq.Strings.String.
+
+Require Import Coq.Structures.Equalities.
+Require Import Coq.Arith.EqNat.
 
 Require Import Ast.
+Require Import Semantics.
+Require Import Store.
 
-Inductive value : expr -> Prop :=
-| v_null : value expr_null
-| v_term : forall n, value (expr_term n)
-.
+Fixpoint eval (f: frame) (e: expr) : frame * nat :=
+  match e with
+  | expr_temp t => (f, t)
 
-Reserved Notation "t1 '==>' t2" (at level 40).
-Inductive step : expr -> expr -> Prop :=
-| E_Seq : forall v e,
-        value v ->
-        expr_seq v e ==> e
-| E_Recover : forall v,
-        value v ->
-        expr_recover v ==> v
-where "e1 '==>' e2" := (step e1 e2).
+  | expr_recover e' => eval f e'
+  | expr_local name =>
+      let t := Frame.alloc_temp f in
+      let f' := Frame.set f (TempId t) (Frame.get f (SourceId name)) in
+      (f', t)
 
-Hint Constructors step.
+  | expr_assign_local name e =>
+      let (f', t) := eval f e in
+      let t' := Frame.alloc_temp f' in
+      let f'' := Frame.set f' (TempId t') (Frame.get f' (SourceId name)) in
+      let f''' := Frame.set f'' (SourceId name) (Frame.get f' (TempId t)) in
+      (f''', t')
+
+  | expr_seq e1 e2 =>
+      let (f', _) := eval f e1
+      in eval f' e2
+  end.
+
+Theorem eval_step: forall f e f' t,
+  (eval f e = (f', t) -> f / e ==>* f' / expr_temp t).
+Proof.
+intros f e.
+generalize dependent f.
+induction e.
++ intros.
+  simpl in H.
+  inversion H.
+  symmetry in H1.
+  symmetry in H2.
+  rewrite H1.
+  rewrite H2.
+  apply multi_refl.
+
++ intros.
+  simpl in H.
+  remember (eval f e1) as E.
+  symmetry in HeqE.
+  destruct E.
+
+  apply multi_concat with (f2 := f0) (e2 := (expr_seq (expr_temp n) e2)).
+  - apply E_SeqN.
+    apply IHe1.
+    exact HeqE.
+  - apply multi_trans with (f2 := f0) (e2 := e2).
+    * apply E_Seq.
+    * apply IHe2.
+      exact H.
+
++ intros.
+  simpl in H.
+  apply multi_concat with (f2 := f') (e2 := expr_recover (expr_temp t)).
+  - apply E_RecoverN.
+    apply IHe.
+    exact H.
+  - apply multi_one.
+    apply E_Recover.
+
++ intros.
+  simpl in H.
+  inversion H.
+  apply multi_one.
+  apply E_Local.
+  reflexivity.
+  reflexivity.
+
++ intros.
+  simpl in H.
+  remember (eval f e) as E.
+  symmetry in HeqE.
+  destruct E.
+  apply multi_concat with (f2 := f0) (e2 := expr_assign_local s (expr_temp n)).
+  - apply E_Asn_LocalN.
+    apply IHe.
+    exact HeqE.
+
+  - apply multi_one.
+    inversion H.
+    apply E_Asn_Local.
+    * reflexivity.
+    * reflexivity.
+
+Qed.
+
