src/Semantics.v
@@ -1,0 +1,126 @@
+Require Import Coq.Arith.EqNat.
+Require Import Coq.Strings.String.
+
+Require Import Ast.
+Require Import Store.
+
+Inductive local_id : Type :=
+| SourceId: string -> local_id
+| TempId: nat -> local_id.
+
+Module local_id_eq.
+  Definition t := local_id.
+  Definition eqb x y : bool :=
+    match x, y with
+    | SourceId x', SourceId y' => if string_dec x' y' then true else false
+    | TempId x', TempId y' => beq_nat x' y'
+    | _, _ => false
+    end.
+End local_id_eq.
+
+Inductive value : Type :=
+| v_null: value
+| v_addr: nat -> value.
+
+Module value_default.
+  Definition t := value.
+  Definition default := v_null.
+End value_default.
+
+
+Module Frame.
+  Include Store local_id_eq value_default.
+  Definition alloc_temp (st: store) : nat :=
+    List.length st.
+End Frame.
+
+Definition frame := Frame.store.
+
+Reserved Notation "f1 / e1 '==>' f2 / e2"
+  (at level 40, e1 at level 39, f2 at level 39).
+
+Inductive step : frame * expr -> frame * expr -> Prop :=
+| E_Seq : forall f t e,
+    f / expr_seq (expr_temp t) e ==> f / e
+
+| E_Recover : forall f t,
+    f / expr_recover (expr_temp t) ==> f / (expr_temp t)
+
+| E_Local : forall f t f' name,
+    t = Frame.alloc_temp f ->
+    f' = Frame.set f (TempId t) (Frame.get f (SourceId name)) ->
+    f / expr_local name ==> f' / expr_temp t
+
+| E_Asn_Local : forall f f' t t' name,
+    t' = Frame.alloc_temp f ->
+    f' = Frame.set (Frame.set f (TempId t') (Frame.get f (SourceId name)))
+              (SourceId name) (Frame.get f (TempId t)) ->
+    f / expr_assign_local name (expr_temp t) ==> f' / expr_temp t'
+
+| E_Seq1 : forall f f' e1 e1' e2,
+    f / e1 ==> f' / e1' ->
+    f / expr_seq e1 e2 ==> f' / expr_seq e1' e2
+
+| E_Recover1 : forall f f' e e',
+    f / e ==> f' / e' ->
+    f / expr_recover e ==> f' / expr_recover e'
+
+| E_Asn_Local1 : forall f f' name e e',
+    f / e ==> f' / e' ->
+    f / expr_assign_local name e ==> f' / expr_assign_local name e'
+
+where "f1 / e1 '==>' f2 / e2" := (step (f1,e1) (f2,e2)).
+
+Reserved Notation "f1 / e1 '==>*' f2 / e2"
+  (at level 40, e1 at level 39, f2 at level 39).
+
+Inductive multistep : frame * expr -> frame * expr -> Prop :=
+| multi_refl : forall f e, multistep (f, e) (f, e)
+
+| multi_trans : forall f1 e1 f2 e2 f3 e3,
+    f1 / e1 ==> f2 / e2 ->
+    f2 / e2 ==>* f3 / e3 ->
+    f1 / e1 ==>* f3 / e3
+where "f1 / e1 '==>*' f2 / e2" := (multistep (f1, e1) (f2, e2)).
+
+Theorem multi_one : forall f1 e1 f2 e2,
+  f1 / e1 ==> f2 / e2 ->
+  f1 / e1 ==>* f2 / e2.
+Proof.
+intros.
+apply multi_trans with (f2 := f2) (e2 := e2).
+exact H.
+apply multi_refl.
+Qed.
+
+Theorem multi_concat : forall f1 e1 f2 e2 f3 e3,
+  f1 / e1 ==>* f2 / e2 ->
+  f2 / e2 ==>* f3 / e3 ->
+  f1 / e1 ==>* f3 / e3.
+Proof.
+  intros.
+  generalize dependent f3.
+  generalize dependent e3.
+  induction H.
+  + intros. exact H0.
+  + intros.
+    apply multi_trans with (f2 := f3) (e2 := e3).
+    exact H.
+    apply IHmultistep.
+    exact H1.
+Qed.
+
+Lemma E_RecoverN : forall f f' e e',
+    f / e ==>* f' / e' ->
+    f / expr_recover e ==>* f' / expr_recover e'.
+Admitted.
+
+Lemma E_SeqN : forall f f' e1 e1' e2,
+    f / e1 ==>* f' / e1' ->
+    f / expr_seq e1 e2 ==>* f' / expr_seq e1' e2.
+Admitted.
+
+Lemma E_Asn_LocalN : forall f f' name e e',
+    f / e ==>* f' / e' ->
+    f / expr_assign_local name e ==>* f' / expr_assign_local name e'.
+Admitted.
