src/Store.v
@@ -1,0 +1,34 @@
+Require Import Coq.Structures.Equalities.
+Require Import Coq.Lists.List.
+
+Module Type HasDefault (Import T: Typ).
+  Parameter Inline(30) default : t.
+End HasDefault.
+
+Module Type Default := Typ <+ HasDefault.
+
+Module Type Eqb := Typ <+ HasEqb.
+
+Module Store (K: Eqb) (V: Default).
+  Definition store := list (K.t * V.t).
+  Definition empty : store := nil.
+
+  Fixpoint get (st: store) (k: K.t) : V.t :=
+    match st with
+    | nil => V.default
+    | (k', v) :: tail =>
+        if K.eqb k k'
+        then v
+        else get tail k
+    end.
+
+  Fixpoint set (st: store) (k: K.t) (v: V.t) : store :=
+    match st with
+    | nil => (k, v) :: nil
+    | (k', v') :: tail =>
+        if K.eqb k k'
+        then (k, v) :: tail
+        else (k', v') :: set tail k v
+    end.
+End Store.
+
