src/main.v
@@ -1,4 +1,3 @@
-Require Import Ast.
 Require Import Eval.
 
 Require Import Coq.extraction.ExtrHaskellBasic.
@@ -6,6 +5,4 @@ Require Import Coq.extraction.ExtrHaskellString.
 Require Import Coq.extraction.ExtrHaskellNatInteger.
 
 Extraction Language Haskell.
-Extraction Library Ast.
-Extraction Library Eval.
-
+Recursive Extraction eval.
